Changing notation

Complexity/Asymptotic.lean
@@ -1,64 +1,167 @@
--- import Complexity.Cost
+import Complexity.Cost
 
--- namespace Complexity
--- open CostFunction
+namespace Complexity
+structure ALE (x y: CostFunction α ℕ) where
+  m: ℕ
+  k: ℕ
+  ale: x ≤ m * y + k
 
--- def Asymptotic (α: Type _): Type _ := Quotient (CostFunction.asymptotic α)
+notation:50 f " ∈ O( " g ")" => ALE f g
 
--- instance: Membership (CostFunction α ℕ) (Asymptotic α) where
---   mem cf o := ∃ (k: ℕ), cf ≤ k * o.out + k
+def ale_of_le {x y: CostFunction α ℕ} (h: x ≤ y): x ∈ O(y) := ⟨1, 0, le_of_le_of_eq h (one_mul _).symm⟩
 
--- def O  (f: CostFunction α ℕ): Asymptotic α := ⟦f⟧
+namespace ALE
 
--- namespace Asymptotic
+variable {x y z: CostFunction α ℕ}
 
--- def out_ale (f: CostFunction α ℕ): (O f).out ≤≤ f := (Quotient.exact ((Quotient.out_eq (O _)))).left
--- def ale_out (f: CostFunction α ℕ): f ≤≤ (O f).out := (Quotient.exact ((Quotient.out_eq (O _)))).right
--- theorem mem_self (f: CostFunction α ℕ): f ∈ O f :=
---   And.right (Quotient.exact ((Quotient.out_eq (O _))))
+def bound (h: x ∈ O(y)): CostFunction α ℕ := h.m * y + h.k
 
--- def mem_def {f: CostFunction α ℕ} {g: Asymptotic α}: f ∈ g → f ≤≤ g.out := id
--- def mem_mk {f g: CostFunction α ℕ} (h: f ∈ O g): f ≤≤ g := Trans.trans (mem_def h) (out_ale _)
+theorem le_bound (h: x ∈ O(y)): x ≤ h.bound := h.ale
 
--- noncomputable def k_of_mem {f: CostFunction α ℕ} {g: Asymptotic α} (h: f ∈ g): ℕ := Classical.choose h
--- noncomputable def k_of_mk (f: CostFunction α ℕ): ℕ := Classical.choose (out_ale f)
--- noncomputable def k_of_mk' (f: CostFunction α ℕ): ℕ := Classical.choose (ale_out f)
--- noncomputable def k_of_mem_mk {f g: CostFunction α ℕ} (h: f ∈ O g): ℕ := Classical.choose (mem_mk h)
+def refl: x ∈ O(x) := ale_of_le (le_refl _)
 
--- theorem k_of_mem_sound {f: CostFunction α ℕ} {g: Asymptotic α} (h: f ∈ g): f ≤ (k_of_mem h * g.out) + (k_of_mem h) := Classical.choose_spec h
--- theorem k_of_mk_sound (f: CostFunction α ℕ): (O f).out ≤ (k_of_mk f * f) + (k_of_mk f) :=
---   Classical.choose_spec (out_ale f)
--- theorem k_of_mk'_sound (f: CostFunction α ℕ): f ≤ (k_of_mk' f * (O f).out) + (k_of_mk' f) :=
---   Classical.choose_spec (ale_out f)
--- theorem k_of_mem_mk'_sound {f g: CostFunction α ℕ} (h: f ∈ O g): f ≤ (k_of_mem_mk h * g) + (k_of_mem_mk h) :=
---   Classical.choose_spec (mem_mk h)
+def trans (hxy: x ∈ O(y)) (hyz: y ∈ O(z)): x ∈ O(z) where
+  m := hxy.m * hyz.m
+  k := hxy.m * hyz.k + hxy.k
+  ale := le_trans hxy.le_bound
+    (le_of_le_of_eq (add_le_add (le_of_le_of_eq
+      (mul_le_mul (le_refl _) hyz.le_bound (zero_le _) (zero_le _))
+      ((left_distrib _ _ _).trans
+        (congrArg₂ _ (mul_assoc _ _ _).symm rfl)))
+      (le_refl _))
+      (add_assoc _ _ _))
 
--- instance: PartialOrder (Asymptotic α) where
---   le := Quotient.lift₂ (CostFunction.ALE) (λ _ _ _ _ ha hb ↦
---     eq_iff_iff.mpr ⟨
---       λ h ↦ Trans.trans ha.right (Trans.trans h hb.left),
---       λ h ↦ Trans.trans  ha.left (Trans.trans h hb.right) ⟩)
---   le_refl a := Quotient.out_eq a ▸ refl (r := CostFunction.ALE) _
---   le_trans a b c := Quotient.out_eq a ▸ Quotient.out_eq b ▸ Quotient.out_eq c ▸ Trans.trans (r := CostFunction.ALE) (s := CostFunction.ALE)
---   le_antisymm a b := by exact Quotient.out_eq a ▸ Quotient.out_eq b ▸ λ hab hbc ↦ Quotient.sound (s := CostFunction.asymptotic α) (And.intro hab hbc)
+def ale_of_le_of_ale (hxy: x ≤ y) (hyz: y ∈ O(z)): x ∈ O(z) := trans (ale_of_le hxy) hyz
 
--- theorem o1_le (g: Asymptotic α): O 1 ≤ g := flip le_of_le_of_eq (Quotient.out_eq g) ⟨_, λ _ ↦ (Nat.le_add_left _ _)⟩
+def add_ale (hxz: x ∈ O(z)) (hyz: y ∈ O(z)): x + y ∈ O(z) where
+  m := hxz.m + hyz.m
+  k := hxz.k + hyz.k
+  ale :=
+    le_of_le_of_eq (add_le_add hxz.ale hyz.ale)
+      (add_left_comm (hyz.m * z) _ _ ▸
+      add_assoc (hxz.m * z) _ _ ▸
+      add_assoc (hyz.m * z) _ _ ▸
+      add_comm (hyz.m * z) _ ▸
+      right_distrib _ _ z ▸
+      CostFunction.const_add_const _ _ ▸
+      rfl)
 
--- instance: Add (Asymptotic α) where
---   add := Quotient.lift₂ (λ a b ↦ ⟦a + b⟧) (
---     λ _ _ _ _ ha hb ↦ Quotient.sound ⟨
---       CostFunction.add_ale_add ha.left hb.left,
---       CostFunction.add_ale_add ha.right hb.right ⟩)
+def const_ale (n: ℕ) (f: CostFunction α ℕ): n ∈ O(f) where
+  m := 0
+  k := n
+  ale := le_add_left (le_refl _)
 
--- instance: Mul (Asymptotic α) where
---   mul := Quotient.lift₂ (λ x y ↦ ⟦CostFunction.mul' x y⟧) (
---     λ _ _ _ _ hx hy ↦ Quotient.sound ⟨
---       CostFunction.mul'_ale_mul' hx.left hy.left,
---       CostFunction.mul'_ale_mul' hx.right hy.right⟩)
 
--- def flatMap (f: α → Option β): Asymptotic β → Asymptotic α :=
---   Quotient.lift (λ x ↦ ⟦ x.flatMap f ⟧) ( λ _ _ h ↦ Quotient.sound ⟨
---       CostFunction.flatMap_ale_flatMap h.left _,
---       CostFunction.flatMap_ale_flatMap h.right _⟩)
--- end Asymptotic
--- end Complexity
+end ALE
+
+
+-- instance : IsPreorder (CostFunction α ℕ) (. ≤≤ .) where
+--   refl _ :=  ⟨_, le_add_right (le_of_eq (one_mul _).symm) ⟩
+--   trans _ _ _ hab hbc := hab.elim (hbc.elim λ k₁ h₁ k₀ h₀ ↦
+--     ⟨ k₀ * k₁ + k₀,
+--       h₀.trans (const_add_const (α := α) (k₀ * k₁) k₀ ▸ add_assoc (G := CostFunction α ℕ) _ _ _ ▸
+--         (add_le_add_right (const_mul_const (α := α) k₀ k₁ ▸
+--         mul_add_one (α := CostFunction α ℕ) k₀ k₁ ▸
+--         mul_assoc (G := CostFunction α ℕ) k₀ _ _ ▸
+--         left_distrib (R := CostFunction α ℕ) k₀ _ k₁ ▸
+--           mul_le_mul_of_nonneg_left
+--             (h₁.trans (add_le_add_right
+--               (mul_le_mul_of_nonneg_right (le_add_right (le_refl _))
+--               (zero_le _)) _))
+--             (zero_le _)) _))⟩)
+
+-- theorem add_ale_add {a x b y: CostFunction α ℕ} (hax: a ≤≤ x) (hby: b ≤≤ y): a + b ≤≤ x + y := by
+--   apply hax.elim
+--   apply hby.elim
+--   intro k₁ h₁ k₀ h₀
+--   refine ⟨ k₀ + k₁, ?hha ⟩
+--   refine const_add_const (α := α) k₀ k₁ ▸ ?hhb
+--   refine add_assoc (G := CostFunction α ℕ) _ _ _ ▸ ?hhc
+--   refine left_distrib (R := CostFunction α ℕ)  _ _ _ ▸ ?hhd
+--   refine add_right_comm (G := CostFunction α ℕ) _ k₀ _ ▸ ?hhe
+--   refine add_assoc (G := CostFunction α ℕ) _ _ _ ▸ ?hhf
+--   apply add_le_add
+--   apply le_trans h₀
+--   apply add_le_add_right
+--   apply mul_le_mul_of_nonneg_right
+--   apply le_add_right
+--   apply le_refl
+--   apply zero_le
+--   apply le_trans h₁
+--   apply add_le_add_right
+--   apply mul_le_mul_of_nonneg_right
+--   apply le_add_left
+--   apply le_refl
+--   apply zero_le
+
+-- theorem mul_le_mul' {a x: CostFunction α ℕ}: a * x ≤ mul' a x :=
+--   mul_le_mul (le_add_right (le_refl _)) (le_add_right (le_refl _)) (zero_le _) (zero_le _)
+
+-- theorem mul'_ale_mul' {a x b y: CostFunction α ℕ} (hax: a ≤≤ x) (hby: b ≤≤ y): mul' a b ≤≤ mul' x y := by
+--   apply hax.elim
+--   apply hby.elim
+--   intro k₁ h₁ k₀ h₀
+--   use (k₁ + 1) * (k₀ + 1)
+--   apply le_trans
+--   apply mul'_le_mul'
+--   apply h₀
+--   apply h₁
+--   unfold mul'
+--   simp [add_def, mul_def]
+--   ring_nf
+--   simp [add_assoc]
+--   apply add_le_add
+--   apply one_le_two
+--   apply add_le_add
+--   apply le_mul_of_pos_right
+--   apply one_le_two
+--   apply add_le_add_left
+--   apply add_le_add_left
+--   apply add_le_add_left
+--   apply le_add_left
+--   apply add_le_add
+--   apply le_mul_of_pos_right
+--   apply one_le_two
+--   apply add_le_add_left
+--   apply le_add_left
+--   apply le_add_left
+--   apply le_add_left
+--   apply le_add_left
+--   apply le_add_left
+--   apply add_le_add
+--   apply le_mul_of_pos_right
+--   apply one_le_two
+--   apply le_add_right
+--   apply le_refl _
+
+-- theorem mul_ale_mul_of_const_left {a b: CostFunction α ℕ} (h: a ≤≤ b): (n: ℕ) → (n:CostFunction α ℕ) * a ≤≤ (n:CostFunction α ℕ) * b
+-- | 0 => natZero_mul a ▸ natZero_mul b ▸ refl _
+-- | n+1 => by
+--   apply h.elim
+--   intro k h
+--   refine ⟨ n * k + k, ?hha⟩
+--   apply le_trans
+--   apply mul_le_mul_of_nonneg_left h (zero_le _)
+--   simp
+--   ring_nf
+--   apply add_le_add_right
+--   apply add_le_add_right
+--   apply le_add_right
+--   apply add_le_add_left
+--   intro
+--   rw [mul_def (y := 2)]
+--   apply Nat.le_mul_of_pos_right
+--   apply Nat.zero_lt_succ
+
+-- instance asymptotic (α: Type _): Setoid (CostFunction α ℕ) where
+--   r x y := x ≤≤ y ∧ y ≤≤ x
+--   iseqv.refl _ := ⟨ refl _, refl _ ⟩
+--   iseqv.symm h := ⟨h.right, h.left⟩
+--   iseqv.trans hxy hyz := ⟨ Trans.trans hxy.left hyz.left, Trans.trans hyz.right hxy.right ⟩
+
+-- theorem flatMap_ale_flatMap {x y: CostFunction β ℕ} (h: x ≤≤ y) (f: α → Option β):
+--     x.flatMap f ≤≤ y.flatMap f := h.imp λ k hk a ↦
+--   match ha:f a with
+--   | none => flatMap_none ha x ▸ Nat.zero_le _
+--   | some _ => by simpa [add_def, mul_def, flatMap_some ha x, flatMap_some ha y] using hk _
+end Complexity
