HMem/Complexity/Basic.lean
@@ -1,6 +1,5 @@
 import HMem.Encoding.Basic
-import HMem.Trace.TracedProgram
-import HMem.Trace.Sound
+import HMem.Trace.Cost
 import Complexity.Basic
 import HMem.Complexity.Def
 
@@ -9,9 +8,15 @@ import HMem.Complexity.Def
 
 namespace HMem.Complexity
 
-instance [Complexity.Encoding α Memory]: Program.HasTrace ↿(@List.cons α) where
+instance [Complexity.Encoding α Memory]: Program.HasCost ↿(@List.cons α) where
   program := [ .setv 0 true ]
   size _ := 0
   sound | (_, _) => by simp
+  cost := 1
+  cost_le := Complexity.ALE.ale_of_le_of_ale
+    (Program.splitTimeCost _)
+    (Complexity.ALE.add_ale
+      (Complexity.ALE.const_ale _ _)
+      (Program.localTimeCost_const _))
 
 end HMem.Complexity
